\documentclass{article}
\usepackage{amsmath}
\usepackage{amssymb}
\begin{document}
\noindent Proove that $\forall n \in \mathbb{N}, \sum_{k=1}^{n}k^2 =
\frac{n(n+1)(2n+1)}{6}$\\

\noindent Proof:\\
Let $n = 0, P(0)$ is true.\\
Suppose $\forall n \in \mathbb{N}, \sum_{k=1}^{n}k^2 =
\frac{n(n+1)(2n+1)}{6}$\\
$\Rightarrow \sum_{k=1}^{n+1}k^2 = \frac{n(n+1)(2n+1)}{6} + (n+1)^2$\\
$\Rightarrow \sum_{k=1}^{n+1}k^2 = 
\frac{(n+1)[n(2n+1)+6(n+1)]]}{6}$\\
$\Rightarrow \sum_{k=1}^{n+1}k^2 = 
\frac{(n+1)[n(2n+7) + 6]}{6}$\\
$\Rightarrow \sum_{k=1}^{n+1}k^2 = 
\frac{(n+1)[n(2n+3) + 2(2n + 3)]}{6}$\\
$\Rightarrow \sum_{k=1}^{n+1}k^2 = 
\frac{(n+1)(n+2)(2n+3)}{6}$\\

\noindent Proove that $\forall n \in \mathbb{N}, \sum_{k=1}^{n}k^3 = 
\frac{[n(n+1)]^2}{4}$\\

\noindent Proof:\\
Let $n = 0, P(0)$ is true.\\
Suppose $\forall n \in \mathbb{N}, \sum_{k=1}^{n}k^3 = \frac{[n(n+1)]^2}{4}$\\
$\Rightarrow \sum_{k=1}^{n+1}k^3 = \frac{n(n+1)^2 + 4(n+1)^3}{4}$\\
$\Rightarrow \sum_{k=1}^{n+1}k^3 = \frac{(n+1)^2(n^2 + 4(n+1))]}{4}$\\
$\Rightarrow \sum_{k=1}^{n+1}k^3 = \frac{[(n+1)(n+2)]^2}{4}$
\end{document}