\documentclass{article}
\begin{document}
\noindent Let $f: E \rightarrow F $ and a family
of F, $(B_i)_{i \in I} $. Proove that\\
\[
f^{-1}(\bigcap_{i \in I}B_i) =
\bigcap_{i \in I}f^{-1}(B_i)
\]

\noindent Let $x \in  f^{-1}(\bigcap_{i \in I}B_i)$\\
$\Rightarrow \exists y \in  \bigcap_{i \in I}B_i \ |
\ f(x) = y$\\
$\Rightarrow \forall i \in I, x \in f^{-1}(B_i)$\\
$\Rightarrow \forall i \in I, x \in 
\bigcap_{i \in I}f^{-1}(B_i)$\\
$\Rightarrow f^{-1}(\bigcap_{i \in I}B_i) \subset 
\bigcap_{i \in I}f^{-1}(B_i)
$\\

\noindent Let $x \in \bigcap_{i \in I}f^{-1}(B_i)$\\
$\Rightarrow \exists y, \forall i \in I, y \in B_i$
and $ f(x) = y$\\
$\Rightarrow y \in \bigcap_{i \in I}B_i$\\
$\Rightarrow x \in f^{-1}(\bigcap_{i \in I}B_i)$\\
$\Rightarrow f^{-1}(\bigcap_{i \in I}B_i) 
\supset \bigcap_{i \in I}f^{-1}(B_i)$
\end{document}