\documentclass{article}
\begin{document}
\noindent Consider A, B, C. Compare those sets:\\
1. $A \cap (B \cup C) $ and $(A \cap B) \cup (A \cap C)$\\
2. $A \cup (B \cap C) $ and $(A \cup B) \cap (A \cup C)$\\

\noindent 1. Let $x \in A \cap (B \cup C) $\\
$\Rightarrow x \in A$ and ($ x \in B$ or $x \in C)$\\
Applying the rule of replacement in classical logic\\
$\Rightarrow (x \in A$ and $x \in B)$ or $(x \in A$ and $x \in C)$\\
$\Rightarrow x \in (A \cap B) \cup (A \cap C)$\\

\noindent 2. Let $x \in A \cup (B \cap C)$\\
$\Rightarrow (x \in A$  or $x \in B)$ and $ (x \in A$ or $x \in C)$\\
$\Rightarrow x \in (A \cup B) \cap (A \cup C)$\\

\end{document}
