\documentclass{article}
\begin{document}
\noindent
Let $x \in f^{-1}(B_1) $ and $ B_1 \subset B_2 $\\
$\Rightarrow \exists y \in B_2 \ | \ f(x) = y $\\
$\Rightarrow  x \in f^{-1}(B_2)$\\
$\Rightarrow f^{-1}(B_1) \subset f^{1}(B_2)$\\

\noindent
Let $x \in f^{-1}{B_1 \cap B_2} $\\
$\iff \exists y \in B_1 \cap B_2 \ | \ f(x) = y $\\
$\iff x \in f^{-1}(B_1) $ and
$ x \in f^{-1}(B_2) $\\
$\iff x \in f^{-1}(B_1) \cap f^{-1}(B_2) $\\
$\iff f^{-1}{B_1 \cap B_2} =
 f^{-1}(B_1) \cap f^{-1}(B_2) $\\

\noindent
Let $y \in f(A_1) $ and $ A_1 \subset A_2 $\\
$\Rightarrow \exists x \in A_1 \ | \ f(x) = y $ \\
$\Rightarrow y \in f(A_2)$\\
$\Rightarrow f(A_1) \subset f(A_2)$\\

\noindent
Let $y \in f(f^{-1}(B_1))$\\
$\Rightarrow \exists x \in f^{-1}(B_1) \ | \ f(x) = y$\\
$\Rightarrow y \in B_1 $\\
$\Rightarrow f(f^{1}(B_1) \subset B_1 $\\

\noindent
Let $x \in A_1$\\
$\Rightarrow \exists y \in f(A) \ | \ f(x) = y$\\
$\Rightarrow x \in f^{-1}(f(A)) $\\
$\Rightarrow A_1 \subset f^{-1}(f(A)) $\\
\end{document}