\documentclass{article}
\usepackage{amssymb}
\begin{document}
\noindent Let $(A, B) \in P(E)^2$\\
We define $A \Delta B = (A \cup B) \setminus (A \cap B)$\\
Express $ \chi_{(A \cup B) \setminus (A \cap B)} $ in function of $ \chi_A$ and $\chi_B$\\

\noindent
$ \chi_{A \Delta B}  = \chi_{(A\cup B)\cap (E \setminus (A\cap B)}$\\
$ =  (\chi_{A} + \chi_{B} - \chi_{A}\chi_{B}) * (1 - \chi_{A}\chi_{B})$\\
$ = \chi_{A} + \chi_{B} - \chi_{A}^2\chi_{B} - \chi_{A}\chi_{B}^2 + (\chi_{A}\chi_{B})^2 \ - \chi_{A}\chi_{B}$\\\\
Knowing that $\chi_{Y}^2 = \chi_{Y}, \forall Y $ a set\\
$=> \chi_{A\Delta B} = (\chi_{A} - \chi_{B})^2$\\

\noindent $\chi_{(A\Delta B) \Delta C} =
(\chi_{A\Delta B} - \chi_{C})^2$\\
$= ((\chi_{A} - \chi_{B})^2 - \chi_C)^2 $\\
$= \chi_A + \chi_{B} + \chi_C - 2\chi_A\chi_B - 2\chi_C\chi_A - 2\chi_C\chi_B + 4\chi_C\chi_B\chi_A $\\
$= (\chi_B - \chi_C)^2 + \chi_A^2 - 2\chi_A(\chi_B - \chi_C)^2$\\
$= (\chi_A - \chi_{B\Delta C})^2$\\
$= \chi_{A\Delta (B\Delta C)}$\\
Then, $A\Delta(B\Delta C) = (A\Delta B) \Delta C$
\end{document}