\documentclass{article}
\begin{document}
\noindent Let $E$ be a set and $(A_i)_{i\in I}$. Proove
that:\\
\[
E \setminus (\bigcap_{i \in I}A_i) =
\bigcup_{i \in I}(E \setminus A_i)
\]
\[
E \setminus (\bigcup_{i \in I}A_i) =
\bigcap_{i \in I}(E \setminus A_i)
\]\\

\noindent Let $x \in E \setminus (\bigcap_{i \in I}A_i)$\\
$\iff x \in E $ and $(x \notin A_{i_1}  $ or
$ x \notin A_{i_2} $ or \dots \ or $ x \notin A_{i_n})$\\
$\iff (x \notin E $ and $ x \notin A_{i_1}) $ or
$(x \notin E $ and $ x \notin A_{i_2}) $ or \dots\  or
$(x \notin E $ and $ x \notin A_{i_n})$
$\iff  x \in \bigcup_{i \in I}(E \setminus A_i)$\\
$\iff E \setminus (\bigcap_{i \in I}A_i) =
\bigcup_{i \in I}(E \setminus A_i)$\\


\noindent Let $x \in E \setminus (\bigcup_{i \in I}A_i)$\\
$\iff x \in E $ and $(x \notin A_{i_1}  $ and
$ x \notin A_{i_2} $ and \dots \ and $ x \notin A_{i_n})$\\
$\iff x \in \bigcap_{i \in I}(E \setminus A_i)$\\
$E \setminus (\bigcup_{i \in I}A_i) =
\bigcap_{i \in I}(E \setminus A_i)$
\end{document}