\documentclass{article}
\usepackage{amssymb}
\begin{document}
\noindent Let $f \in F^E$ and $g \in G^F$\\
- If $f$ and $g$ are injective, then $g \circ f$ is injective;\\
Proof:\\
Let $ (x, x') \in E^2$ | $ g \circ f(x) = g \circ f(x'1) $;\\
$\Rightarrow f(x) = f(x')$ because $g$ is injective\\
$\Rightarrow x = x' $ because $f$ is injective\\
$\Rightarrow (\forall (x, x') \in E^2, g\circ
f(x) = g \circ f(x')\Rightarrow  x = x')$\\\\

\noindent - If $f$ and $g$ are surjective, then $g \circ f$ is surjective;\\
Proof:\\
Let $ y \in G $\\
$\Rightarrow \exists \alpha \in F $ | $ g(\alpha) = y$\\
$\Rightarrow \exists x \in E $ | $ f(x) = \alpha$ and $g(f(x)) = y$\\
$\Rightarrow g \circ f $ is surjective;\\\\

\noindent
- If $g \circ f$ is injective, then $f$ is injective;\\
Proof:\\
Suppose $f$ is not injective\\
$\Rightarrow \exists (x, x') \in E^2$ | $ f(x) = f(x') $
and $ x \neq x' $\\
$\Rightarrow \exists (x, x') \in E^2$ | $ g(f(x)) = f(x') $
and $ x \neq x' $\\\\

\noindent If $g \circ f$ is surjective, then $g$ is surjective\\
Suppose $g$ is not surjective\\
$\Rightarrow \exists y \in G$ , $\nexists \alpha \in F$ | $ g(\alpha) = y$\\
$\Rightarrow $ (if $\exists x \in E $ | $ f(x) = \alpha \Rightarrow 
\exists y \in G,\  \nexists x \in E $ | $ g(f(x)) = y)$ or
(if $\nexists x \in E $ | $ f(x) = \alpha \Rightarrow
\exists y \in G,\ \nexists x \in E $ | $ g(f(x)) = y)$

\end{document}
